cedar-dafny/thm/basic.dfy
@@ -5,61 +5,38 @@ module basic {
   import opened def.core
   import opened def.engine
 
-  lemma DefaultDeny(query: Query, store: Store)
-    requires // If the policy set is empty, then
-      |store.policies.policies| == 0
-    ensures // every request is denied.
-      Authorizer(query, store).isAuthorized().decision == Deny
-  { }
-
-  lemma ImplicitDeny(query: Query, store: Store)
-    requires // If no permit policy is in force, then
-      forall p |
-        p in store.policies.policies.Keys &&
-        store.policies.policies[p].effect == Permit ::
-        !Authorizer(query, store).isInForce(p)
-    ensures // the request is denied.
-      Authorizer(query, store).isAuthorized().decision == Deny
-  { }
-
-  lemma ForbidTrumpsPermit(query: Query, store: Store)
-    requires // If some forbid policy is in force, then
+  lemma ForbidTrumpsPermit(request: Request, store: Store)
+    requires // If some forbid policy is satisfied, then
       exists f ::
         f in store.policies.policies.Keys &&
         store.policies.policies[f].effect == Forbid &&
-        Authorizer(query, store).isInForce(f)
+        Authorizer(request, store).satisfied(f)
     ensures // the request is denied.
-      Authorizer(query, store).isAuthorized().decision == Deny
+      Authorizer(request, store).isAuthorized().decision == Deny
   {
-    var f :| f in Authorizer(query, store).forbids();
+    var f :| f in Authorizer(request, store).forbids();
   }
 
   // A request is explicitly permitted when there is at least one permit policy
-  // that is in force and no forbid policies are in force.
-  ghost predicate IsExplicitlyPermitted(query: Query, store: Store) {
-    (exists p ::
-       p in store.policies.policies.Keys &&
-       store.policies.policies[p].effect == Permit &&
-       Authorizer(query, store).isInForce(p)) &&
-    (forall f |
-       (f in store.policies.policies.Keys &&
-        store.policies.policies[f].effect == Forbid) ::
-       !Authorizer(query, store).isInForce(f))
+  // that is satisfied.
+  predicate IsExplicitlyPermitted(request: Request, store: Store) {
+    exists p ::
+      p in store.policies.policies.Keys &&
+      store.policies.policies[p].effect == Permit &&
+      Authorizer(request, store).satisfied(p)
   }
 
-  lemma AllowedIffExplicitlyPermitted(query: Query, store: Store)
-    ensures // A request is allowed if and only if it is explictly permitted.
-      Authorizer(query, store).isAuthorized().decision == Allow <==>
-      IsExplicitlyPermitted(query, store)
-  {
-    var authz := Authorizer(query, store);
-    if IsExplicitlyPermitted(query, store) {
-      var p :| p in Authorizer(query, store).permits();
-    } else {
-      if Authorizer(query, store).permits() != {} {
-        var f :| f in Authorizer(query, store).forbids();
-      }
-    }
-  }
+  lemma AllowedIfExplicitlyPermitted(request: Request, store: Store)
+    ensures // A request is allowed only if it is explictly permitted.
+      Authorizer(request, store).isAuthorized().decision == Allow ==>
+        IsExplicitlyPermitted(request, store)
+  { }
+
+  // DefaultDeny is the contrapositive of AllowedIfExplicitlyPermitted
+  lemma DefaultDeny(request: Request, store: Store)
+    ensures // If not explicitly permitted, a request is denied
+      !IsExplicitlyPermitted(request,store) ==>
+        Authorizer(request, store).isAuthorized().decision == Deny
+  { }
 
 }
