cedar-dafny/validation/ext.dfy
@@ -11,4 +11,6 @@ module validation.ext {
   {
     decimal.register() + ipaddr.register()
   }
+
+  const extFunTypes: map<base.Name, ExtFunType> := register();
 }
